modify interpreter to accomodate TRaise

shift-reset/interpreter/interpreter.v
@@ -1,5 +1,5 @@
 From Stdlib Require Import String ZArith.
-From shift_reset.core Require Import syntax env kont loc var.
+From shift_reset.core Require Import syntax env ident kont loc.
 From shift_reset.interpreter Require Import ierror iheap imonad.
 
 Local Open Scope string_scope.
@@ -7,37 +7,37 @@ Local Open Scope Z_scope.
 Local Open Scope imonad_scope.
 Local Unset Elimination Schemes.
 
-Inductive iresult2S : Type :=
-| R2SReturn : val -> iresult2S
-| R2SBubble : (val -> imonad iresult2C) -> kont2C -> iresult2S
-with iresult2C : Type :=
-| R2CReturn : val -> iresult2C
-| R2CBubble : (val -> imonad iresult2S) -> kont2S -> iresult2C.
+Inductive iresult : Type :=
+| RReturn : val -> iresult
+| RShift : (val -> imonad iresult) -> kont2S -> iresult
+| RControl : (val -> imonad iresult) -> kont2C -> iresult
+| RRaise : exn -> iresult.
 
-Inductive iresult3 : Type :=
-| R3Return : val -> iresult3
-| R3BubbleS : (val -> imonad iresult2S) -> kont2S -> iresult3
-| R3BubbleC : (val -> imonad iresult2C) -> kont2C -> iresult3.
-
-Definition handle_R3BubbleS (r : iresult3) : imonad iresult2S :=
+Definition handle_RShift (r : iresult) : imonad iresult :=
   match r with
-  | R3Return v => imonad_pure (R2SReturn v)
-  | R3BubbleS f ks => f (VKontS ks)
-  | R3BubbleC f kc => imonad_pure (R2SBubble f kc)
+  | RShift f ks => f (VKontS ks)
+  | _ => imonad_pure r
   end.
 
-Definition handle_R3BubbleC (r : iresult3) : imonad iresult2C :=
+Definition handle_RControl (r : iresult) : imonad iresult :=
   match r with
-  | R3Return v => imonad_pure (R2CReturn v)
-  | R3BubbleS f ks => imonad_pure (R2CBubble f ks)
-  | R3BubbleC f kc => f (VKontC kc)
+  | RControl f kc => f (VKontC kc)
+  | _ => imonad_pure r
   end.
 
-Definition unwrap_R3Return (r : iresult3) : imonad val :=
+Definition unwrap_RReturn (r : iresult) : imonad val :=
   match r with
-  | R3Return v => imonad_pure v
-  | R3BubbleS _ _ => imonad_throw (ControlError "undelimited shift")
-  | R3BubbleC _ _ => imonad_throw (ControlError "undelimited control")
+  | RReturn v => imonad_pure v
+  | RShift _ _ => imonad_throw (ControlError "undelimited shift")
+  | RControl _ _ => imonad_throw (ControlError "undelimited control")
+  | RRaise _ => imonad_throw (ControlError "unhandled exception")
+  end.
+
+Definition unwind_result (k : kont1) (r : iresult) : iresult :=
+  match r with
+  | RShift f ks => RShift f (K2SSnoc ks k)
+  | RControl f kc => RControl f (K2CSnoc kc k)
+  | _ => r
   end.
 
 Definition unwrap_VInt (v : val) : imonad Z :=
@@ -66,7 +66,7 @@ Definition interpret_atom (a : atom) : imonad val :=
   | AVar x =>
       env <- imonad_ask_env;
       match env_lookup x env with
-      | None => imonad_throw (NameError (var_car x))
+      | None => imonad_throw (NameError (ident_car x))
       | Some v => imonad_pure v
       end
   end.
@@ -128,6 +128,9 @@ Definition interpret_inl (a : atom) : imonad val :=
 Definition interpret_inr (a : atom) : imonad val :=
   VInr <$> interpret_atom a.
 
+Definition interpret_exn (x : ident) (a : atom) : imonad val :=
+  imonad_map (fun v => VExn (Exn x v)) (interpret_atom a).
+
 Definition interpret_ref (a : atom) : imonad val :=
   v <- interpret_atom a;
   h <- imonad_get_heap;
@@ -161,21 +164,21 @@ Definition interpret_free (a : atom) : imonad val :=
   | Some h' => VUnit <$ imonad_set_heap h'
   end.
 
-Definition interpret_let : (env -> imonad iresult3) -> imonad iresult3 :=
+Definition interpret_let : (env -> imonad iresult) -> imonad iresult :=
   imonad_bind imonad_ask_env.
 
-Definition interpret_if (a : atom) (m1 m2 : imonad iresult3) : imonad iresult3 :=
+Definition interpret_if (a : atom) (m1 m2 : imonad iresult) : imonad iresult :=
   b <- interpret_atom a >>= unwrap_VBool;
   if b then m1 else m2.
 
-Definition interpret_split (a : atom) (f : val -> val -> imonad iresult3) : imonad iresult3 :=
+Definition interpret_split (a : atom) (f : val -> val -> imonad iresult) : imonad iresult :=
   v <- interpret_atom a;
   match v with
   | VPair v1 v2 => f v1 v2
   | _ => imonad_throw (TypeError "")
   end.
 
-Definition interpret_case (a : atom) (f1 f2 : val -> imonad iresult3) : imonad iresult3 :=
+Definition interpret_case (a : atom) (f1 f2 : val -> imonad iresult) : imonad iresult :=
   v <- interpret_atom a;
   match v with
   | VInl v' => f1 v'
@@ -183,63 +186,62 @@ Definition interpret_case (a : atom) (f1 f2 : val -> imonad iresult3) : imonad i
   | _ => imonad_throw (TypeError "")
   end.
 
-Definition interpret_reset (k : kont1) (m : imonad iresult3) (f : val -> imonad iresult3) : imonad iresult3 :=
-  r <- m >>= handle_R3BubbleS;
-  match r with
-  | R2SReturn v => f v
-  | R2SBubble f' kc => imonad_pure (R3BubbleC f' (K2CSnoc kc k))
+Definition interpret_reset (k : kont1) (m : imonad iresult) (f : val -> imonad iresult) : imonad iresult :=
+  unwind_result k <$> m >>= handle_RShift.
+
+Definition interpret_prompt (k : kont1) (m : imonad iresult) (f : val -> imonad iresult) : imonad iresult :=
+  unwind_result k <$> m >>= handle_RControl.
+
+Definition interpret_shift (k : kont1) (f : env -> val -> imonad iresult) : imonad iresult :=
+  imonad_map (fun env => RShift (f env >=> handle_RShift) (K2SHead k)) imonad_ask_env.
+
+Definition interpret_control (k : kont1) (f : env -> val -> imonad iresult) : imonad iresult :=
+  imonad_map (fun env => RControl (f env >=> handle_RControl) (K2CHead k)) imonad_ask_env.
+
+Definition interpret_raise (a : atom) : imonad iresult :=
+  v <- interpret_atom a;
+  match v with
+  | VExn exn => imonad_pure (RRaise exn)
+  | _ => imonad_throw (TypeError "")
   end.
 
-Definition interpret_prompt (k : kont1) (m : imonad iresult3) (f : val -> imonad iresult3) : imonad iresult3 :=
-  r <- m >>= handle_R3BubbleC;
-  match r with
-  | R2CReturn v => f v
-  | R2CBubble f' ks => imonad_pure (R3BubbleS f' (K2SSnoc ks k))
-  end.
-
-Definition interpret_shift (k : kont1) (f : env -> val -> imonad iresult3) : imonad iresult3 :=
-  imonad_map (fun env => R3BubbleS (f env >=> handle_R3BubbleS) (K2SHead k)) imonad_ask_env.
-
-Definition interpret_control (k : kont1) (f : env -> val -> imonad iresult3) : imonad iresult3 :=
-  imonad_map (fun env => R3BubbleC (f env >=> handle_R3BubbleC) (K2CHead k)) imonad_ask_env.
-
-Definition with_binder (b : binder) (v : val) (m : imonad iresult3) : imonad iresult3 :=
+Definition with_binder (b : binder) (v : val) (m : imonad iresult) : imonad iresult :=
   match b with
   | BAnon => m
-  | BVar x => imonad_local_env (ECons x v) m
+  | BVar x => imonad_local_env (EnvCons x v) m
   end.
 
-Definition interpret_term1_with (rec : term -> imonad iresult3) (t : term1) (v : val) : imonad iresult3 :=
+Definition interpret_term1_with (rec : term -> imonad iresult) (t : term1) (v : val) : imonad iresult :=
   let (b, t') := t in with_binder b v (rec t').
 
-Definition interpret_term2_with (rec : term -> imonad iresult3) (t : term2) (v1 v2 : val) : imonad iresult3 :=
+Definition interpret_term2_with (rec : term -> imonad iresult) (t : term2) (v1 v2 : val) : imonad iresult :=
   let (b1, b2, t') := t in with_binder b1 v1 (with_binder b2 v2 (rec t')).
 
-Definition interpret_clo1_with (rec : term -> imonad iresult3) (c : clo1) (v : val) : imonad iresult3 :=
+Definition interpret_clo1_with (rec : term -> imonad iresult) (c : clo1) (v : val) : imonad iresult :=
   let (env, t) := c in imonad_local_env (fun _ => env) (interpret_term1_with rec t v).
 
-Definition interpret_clo2_with (rec : term -> imonad iresult3) (c : clo2) (v1 v2 : val) : imonad iresult3 :=
+Definition interpret_clo2_with (rec : term -> imonad iresult) (c : clo2) (v1 v2 : val) : imonad iresult :=
   let (env, t) := c in imonad_local_env (fun _ => env) (interpret_term2_with rec t v1 v2).
 
-Definition interpret_kont1_with (rec : kont1 -> term -> imonad iresult3) (k : kont1) (v : val) : imonad iresult3 :=
+Definition interpret_kont1_with (rec : kont1 -> term -> imonad iresult) (k : kont1) (v : val) : imonad iresult :=
   match k with
-  | K1Nil => imonad_pure (R3Return v)
+  | K1Nil => imonad_pure (RReturn v)
   | K1Cons c k' => interpret_clo1_with (rec k') c v
   end.
 
-Fixpoint interpret_kont2S_with (rec : kont1 -> term -> imonad iresult3) (ks : kont2S) (v : val) : imonad iresult3 :=
+Fixpoint interpret_kont2S_with (rec : kont1 -> term -> imonad iresult) (ks : kont2S) (v : val) : imonad iresult :=
   match ks with
   | K2SHead k => interpret_kont1_with rec k v
   | K2SSnoc ks' k => interpret_prompt k (interpret_kont2S_with rec ks' v) (interpret_kont1_with rec k)
   end.
 
-Fixpoint interpret_kont2C_with (rec : kont1 -> term -> imonad iresult3) (kc : kont2C) (v : val) : imonad iresult3 :=
+Fixpoint interpret_kont2C_with (rec : kont1 -> term -> imonad iresult) (kc : kont2C) (v : val) : imonad iresult :=
   match kc with
   | K2CHead k => interpret_kont1_with rec k v
   | K2CSnoc kc' k => interpret_reset k (interpret_kont2C_with rec kc' v) (interpret_kont1_with rec k)
   end.
 
-Definition interpret_app (rec : kont1 -> term -> imonad iresult3) (k : kont1) (a1 a2 : atom) (f : val -> imonad iresult3) : imonad iresult3 :=
+Definition interpret_app (rec : kont1 -> term -> imonad iresult) (k : kont1) (a1 a2 : atom) (f : val -> imonad iresult) : imonad iresult :=
   v <- interpret_atom a1;
   match v with
   | VFun c => interpret_atom a2 >>= interpret_clo1_with (rec k) c
@@ -273,6 +275,9 @@ Inductive term_graph : kont1 -> term -> Prop :=
 | GTReset k t' : term_graph K1Nil t' -> kont1_graph k -> term_graph k (TReset t')
 | GTControl k t' : (forall env, clo1_graph K1Nil (C1 env t')) -> term_graph k (TControl t')
 | GTPrompt k t' : term_graph K1Nil t' -> kont1_graph k -> term_graph k (TPrompt t')
+| GTExn k x a : kont1_graph k -> term_graph k (TExn x a)
+| GTRaise k a : term_graph k (TRaise a)
+| GTTry k t1 x t2 : term_graph K1Nil t1 -> kont1_graph k -> term_graph k (TTry t1 x t2)
 with term1_graph : kont1 -> term1 -> Prop :=
 | GT1 k b t' : term_graph k t' -> term1_graph k (T1 b t')
 with term2_graph : kont1 -> term2 -> Prop :=
@@ -358,6 +363,9 @@ Proof. inversion 1; auto. Defined.
 Lemma GTPrompt_inv2 k t' : term_graph k (TPrompt t') -> kont1_graph k.
 Proof. inversion 1; auto. Defined.
 
+Lemma GTExn_inv k x a : term_graph k (TExn x a) -> kont1_graph k.
+Proof. inversion 1; auto. Defined.
+
 Lemma GT1_inv k b t' : term1_graph k (T1 b t') -> term_graph k t'.
 Proof. inversion 1; auto. Defined.
 
@@ -393,6 +401,9 @@ Fixpoint build_term_graph_dep (k : kont1) (G : kont1_graph k) (t : term) : term_
   | TReset t' => GTReset (build_term_graph_dep GK1Nil t') G
   | TControl t' => GTControl k (fun env => GC1 env (build_term1_graph_dep GK1Nil t'))
   | TPrompt t' => GTPrompt (build_term_graph_dep GK1Nil t') G
+  | TExn x a => GTExn x a G
+  | TRaise a => GTRaise k a
+  | TTry t1 x t2 => GTTry x t2 (build_term_graph_dep GK1Nil t1) G
   end
 with build_term1_graph_dep (k : kont1) (G : kont1_graph k) (t : term1) : term1_graph k t :=
   match t with
@@ -408,8 +419,8 @@ Definition build_clo1_graph_dep (k : kont1) (G : kont1_graph k) (c : clo1) : clo
   | C1 env t => GC1 env (build_term1_graph_dep G t)
   end.
 
-Fixpoint interpret_term_dep (rec : kont1 -> term -> imonad iresult3) (k : kont1) (t : term) (G : term_graph k t) : imonad iresult3 :=
-  match t return term_graph k t -> imonad iresult3 with
+Fixpoint interpret_term_dep (rec : kont1 -> term -> imonad iresult) (k : kont1) (t : term) (G : term_graph k t) : imonad iresult :=
+  match t return term_graph k t -> imonad iresult with
   | TAtom a => fun G => interpret_atom a >>= interpret_kont1_dep rec (GTAtom_inv G)
   | TFun t' => fun G => interpret_fun t' >>= interpret_kont1_dep rec (GTFun_inv G)
   | TFix t' => fun G => interpret_fix t' >>= interpret_kont1_dep rec (GTFix_inv G)
@@ -431,22 +442,25 @@ Fixpoint interpret_term_dep (rec : kont1 -> term -> imonad iresult3) (k : kont1)
   | TReset t' => fun G => interpret_reset k (interpret_term_dep rec (GTReset_inv1 G)) (interpret_kont1_dep rec (GTReset_inv2 G))
   | TControl t' => fun G => interpret_control k (fun env => interpret_clo1_dep rec (GTControl_inv G env))
   | TPrompt t' => fun G => interpret_prompt k (interpret_term_dep rec (GTPrompt_inv1 G)) (interpret_kont1_dep rec (GTPrompt_inv2 G))
+  | TExn x a => fun G => interpret_exn x a >>= interpret_kont1_dep rec (GTExn_inv G)
+  | TRaise a => fun G => interpret_raise a
+  | TTry t1 x t2 => fun G => imonad_throw (ControlError "todo")
   end G
-with interpret_term1_dep (rec : kont1 -> term -> imonad iresult3) (k : kont1) (t : term1) (G : term1_graph k t) (v : val) : imonad iresult3 :=
-  match t return term1_graph k t -> imonad iresult3 with
+with interpret_term1_dep (rec : kont1 -> term -> imonad iresult) (k : kont1) (t : term1) (G : term1_graph k t) (v : val) : imonad iresult :=
+  match t return term1_graph k t -> imonad iresult with
   | T1 b t' => fun G => with_binder b v (interpret_term_dep rec (GT1_inv G))
   end G
-with interpret_term2_dep (rec : kont1 -> term -> imonad iresult3) (k : kont1) (t : term2) (G : term2_graph k t) (v1 v2 : val) : imonad iresult3 :=
-  match t return term2_graph k t -> imonad iresult3 with
+with interpret_term2_dep (rec : kont1 -> term -> imonad iresult) (k : kont1) (t : term2) (G : term2_graph k t) (v1 v2 : val) : imonad iresult :=
+  match t return term2_graph k t -> imonad iresult with
   | T2 b1 b2 t' => fun G => with_binder b1 v1 (with_binder b2 v2 (interpret_term_dep rec (GT2_inv G)))
   end G
-with interpret_clo1_dep (rec : kont1 -> term -> imonad iresult3) (k : kont1) (c : clo1) (G : clo1_graph k c) (v : val) : imonad iresult3 :=
-  match c return clo1_graph k c -> imonad iresult3 with
+with interpret_clo1_dep (rec : kont1 -> term -> imonad iresult) (k : kont1) (c : clo1) (G : clo1_graph k c) (v : val) : imonad iresult :=
+  match c return clo1_graph k c -> imonad iresult with
   | C1 env t => fun G => imonad_local_env (fun _ => env) (interpret_term1_dep rec (GC1_inv G) v)
   end G
-with interpret_kont1_dep (rec : kont1 -> term -> imonad iresult3) (k : kont1) (G : kont1_graph k) (v : val) : imonad iresult3 :=
-  match k return kont1_graph k -> imonad iresult3 with
-  | K1Nil => fun _ => imonad_pure (R3Return v)
+with interpret_kont1_dep (rec : kont1 -> term -> imonad iresult) (k : kont1) (G : kont1_graph k) (v : val) : imonad iresult :=
+  match k return kont1_graph k -> imonad iresult with
+  | K1Nil => fun _ => imonad_pure (RReturn v)
   | K1Cons c k' => fun G => interpret_clo1_dep rec (GK1Cons_inv G) v
   end G.
 
@@ -461,17 +475,17 @@ Fixpoint build_kont1_graph (k : kont1) : kont1_graph k :=
 Definition build_term_graph (k : kont1) (t : term) : term_graph k t :=
   build_term_graph_dep (build_kont1_graph k) t.
 
-Definition interpret_term_aux (rec : kont1 -> term -> imonad iresult3) (k : kont1) (t : term) : imonad iresult3 :=
+Definition interpret_term_aux (rec : kont1 -> term -> imonad iresult) (k : kont1) (t : term) : imonad iresult :=
   interpret_term_dep rec (build_term_graph k t).
 
-Fixpoint interpret_term (fuel : nat) (k : kont1) (t : term) : imonad iresult3 :=
+Fixpoint interpret_term (fuel : nat) (k : kont1) (t : term) : imonad iresult :=
   match fuel with
   | O => imonad_throw OutOfFuel
   | S fuel' => interpret_term_aux (interpret_term fuel') k t
   end.
 
 Definition run_term (fuel : nat) (t : term) : (ierror + val) * iheap :=
-  imonad_run (interpret_term fuel K1Nil t >>= unwrap_R3Return) ENil iheap_empty.
+  imonad_run (interpret_term fuel K1Nil t >>= unwrap_RReturn) EnvNil iheap_empty.
 
 Definition eval_term (fuel : nat) (t : term) : ierror + val :=
   fst (run_term fuel t).
